We’ll convert your grammar:

[
A_1 → A_3A_2 ;|; A_2A_3
]
[
A_2 → A_3A_3 ;|; A_2A_2 ;|; a
]
[
A_3 → A_2A_2 ;|; b
]

into **Greibach Normal Form (GNF)**, in a clean “Step-by-Step Classroom Board Style” explanation.

---

## ✳️ **Convert the following CFG into GNF**

### Given:

[
A_1 → A_3A_2 ;|; A_2A_3
]
[
A_2 → A_3A_3 ;|; A_2A_2 ;|; a
]
[
A_3 → A_2A_2 ;|; b
]

---

### **Step 1: Check – CNF form or not**

We first check if grammar is in **Chomsky Normal Form (CNF)**.
Each rule is of type:

* ( A \to BC ) ✅ or ( A \to a ) ✅

Hence, **yes**, the grammar is in **CNF form**, so we can now proceed to convert it to **GNF**.

---

### **Step 2: Variable Renaming (for easy tracking)**

Let’s rename variables as:

[
A_1 = A, \quad A_2 = B, \quad A_3 = C
]

So grammar becomes:

[
A → CB ;|; BC
]
[
B → CC ;|; BB ;|; a
]
[
C → BB ;|; b
]

We’ll now apply the **GNF conversion steps** in order:
Start from lowest-numbered variable (here (C)), then (B), then (A).

---

### **Step 3: Convert C to GNF**

Given:
[
C → BB ;|; b
]

Substitute (B → CC ;|; BB ;|; a) into (BB):

[
C → (CC ;|; BB ;|; a)(CC ;|; BB ;|; a) ;|; b
]

Now we only keep productions where **RHS starts with a terminal (a or b)**.

So, the possible derivations that start with terminals:

* ( aCC, aBB, aCB, aBC ) (start with a)
* ( b ) (already terminal)

Therefore:
[
\boxed{C → aCC ;|; aBB ;|; aCB ;|; b}
]
✅ (C) is now in **GNF**.

---

### **Step 4: Convert B to GNF**

Given:
[
B → CC ;|; BB ;|; a
]

Substitute (C → aCC ;|; aBB ;|; aCB ;|; b) into the first (C):

[
B → (aCC ;|; aBB ;|; aCB ;|; b)C ;|; BB ;|; a
]

Now take only the RHSs that start with terminals:

✅ start with `a` or `b`:

[
\boxed{B → aCC ;|; aBB ;|; aCB ;|; bC ;|; a}
]

✅ (B) is now in **GNF**.

---

### **Step 5: Convert A to GNF**

Given:
[
A → CB ;|; BC
]

Substitute (C) and (B) with their GNF forms.

#### For (A → CB):

[
C → aCC ;|; aBB ;|; aCB ;|; b
]
So:
[
CB → (aCC ;|; aBB ;|; aCB ;|; b)B
]
Gives:
[
A → aCCB ;|; aBBB ;|; aCBB ;|; bB
]

#### For (A → BC):

[
B → aCC ;|; aBB ;|; aCB ;|; bC ;|; a
]
and (C → aCC ;|; aBB ;|; aCB ;|; b)

So:
[
BC → (aCC ;|; aBB ;|; aCB ;|; bC ;|; a)(aCC ;|; aBB ;|; aCB ;|; b)
]

Taking only first terminals:

[
A → aCC ;|; aBB ;|; aCB ;|; bC ;|; a
]

Combine both parts:

[
\boxed{
A → aCCB ;|; aBBB ;|; aCBB ;|; bB ;|; aCC ;|; aBB ;|; aCB ;|; bC ;|; a
}
]

✅ (A) is now in **GNF** (all RHS start with a terminal).

---

### **Step 6: Final Result**

Now rename back:
[
A = A_1, \quad B = A_2, \quad C = A_3
]

Final **GNF Grammar**:

[
\boxed{
\begin{aligned}
A_1 &→ aA_3A_3A_2 ;|; aA_2A_2A_2 ;|; aA_3A_2A_2 ;|; bA_2 ;|; aA_3A_3 ;|; aA_2A_2 ;|; aA_3A_2 ;|; bA_3 ;|; a \
A_2 &→ aA_3A_3 ;|; aA_2A_2 ;|; aA_3A_2 ;|; bA_3 ;|; a \
A_3 &→ aA_3A_3 ;|; aA_2A_2 ;|; aA_3A_2 ;|; b
\end{aligned}
}
]

---

### ✅ **Check:**

* Every production starts with a **terminal** (either `a` or `b`)
* No ε-productions
* No unit productions
  Hence the grammar is in **Greibach Normal Form (GNF)** ✔️

